Nemonuri/Executions/ExecutionFragment/Syntax.lean
@@ -1,5 +1,6 @@
 module
 
 public import Nemonuri.Executions.ExecutionFragment.Syntax.Raws
-public import Nemonuri.Executions.ExecutionFragment.Syntax.Projections
 public import Nemonuri.Executions.ExecutionFragment.Syntax.Basic
+public import Nemonuri.Executions.ExecutionFragment.Syntax.Projections
+public import Nemonuri.Executions.ExecutionFragment.Syntax.HasLabel
