Nemonuri/Executions/ExecutionFragment/Syntax/HasLabel.lean
@@ -1,0 +1,105 @@
+module
+
+public import Nemonuri.HasLabel
+public import Nemonuri.Executions.ExecutionFragment.Syntax.Projections
+
+@[expose] public section
+
+namespace Nemonuri.TransitionSystem.ExecutionFragment.SyntaxRaw
+
+open HasLabel
+
+variable {ts: TransitionSystem}
+
+theorem toLabel_eq_toLabelAt : (@SyntaxRaw.toLabel ts) = (toLabelAt Label (SyntaxRaw ts)) := rfl
+
+theorem toSeqLabel_eq_toLabelAt : (@SyntaxRaw.toSeqLabel ts) = (toLabelAt Sequence.Label (SyntaxRaw ts)) := rfl
+
+
+theorem consEllipsis_preserves_seqLabel : HasLabel.Preserves Sequence.Label (@consEllipsis ts) := by
+  apply Preserves.mk _ ?_
+  intro x
+  cases x <;> rfl
+
+protected theorem stepL_preserves_label {s a} : HasLabel.Preserves Label (@stepL ts · s a) := by
+  apply Preserves.mk _ ?_
+  intro x
+  cases x <;> rfl
+
+protected theorem stepL_preserves_seqLabel {s a} : HasLabel.Preserves Sequence.Label (@stepL ts · s a) := by
+  apply Preserves.mk _ ?_
+  intro x
+  cases x <;> rfl
+
+
+
+def stepLFlip (s: ts.S) (a: ts.Act) (tail: SyntaxRaw ts) : SyntaxRaw ts := tail.stepL s a
+
+section StepLFlip
+
+variable {tail: SyntaxRaw ts} {s: ts.S} {a: ts.Act}
+
+@[defeq]
+theorem stepL_eq_stepLFlip : (stepL tail s a) = (stepLFlip s a tail) := rfl
+
+theorem stepLFlip_preserves_label : HasLabel.Preserves Label (stepLFlip s a) := @SyntaxRaw.stepL_preserves_label ts s a
+
+theorem stepLFlip_preserves_seqLabel : HasLabel.Preserves Sequence.Label (stepLFlip s a) := @SyntaxRaw.stepL_preserves_seqLabel ts s a
+
+
+
+theorem stepLFlip_whole_eq_whole_stepLFlip (req: toLabelAt Label (SyntaxRaw ts) tail = .unique)
+  : ((stepLFlip s a tail).whole (stepLFlip_preserves_label.cancel.trans req)) = (tail.whole req).stepL s a := by
+  dsimp [← stepL_eq_stepLFlip]
+  exact stepL_whole_eq_whole_stepL req
+
+@[simp]
+theorem stepLFlip_whole_states_eq_whole_stepLFlip_states (req: toLabelAt Label (SyntaxRaw ts) tail = .unique)
+  : ((stepLFlip s a tail).whole (stepLFlip_preserves_label.cancel.trans req)).states = ((tail.whole req).stepL s a).states :=
+  congrArg _ (stepLFlip_whole_eq_whole_stepLFlip req)
+
+@[simp]
+theorem stepLFlip_whole_actions_eq_whole_stepLFlip_actions (req: toLabelAt Label (SyntaxRaw ts) tail = .unique)
+  : ((stepLFlip s a tail).whole (stepLFlip_preserves_label.cancel.trans req)).actions = ((tail.whole req).stepL s a).actions :=
+  congrArg _ (stepLFlip_whole_eq_whole_stepLFlip req)
+
+end StepLFlip
+
+
+@[defeq, simp]
+theorem unique_toLabelAt {x} : toLabelAt Label (SyntaxRaw ts) (.unique x) = .unique := rfl
+
+@[defeq, simp]
+theorem finites_toLabelAt {x1 x2} : toLabelAt Label (SyntaxRaw ts) (.finites x1 x2) = .finites := rfl
+
+@[defeq, simp]
+theorem infinites_toLabelAt {x} : toLabelAt Label (SyntaxRaw ts) (.infinites x) = .infinites := rfl
+
+
+@[defeq, simp]
+theorem unique_toLabelAt_seq {x} : toLabelAt Sequence.Label (SyntaxRaw ts) (.unique x) = .finite := rfl
+
+@[defeq, simp]
+theorem finites_toLabelAt_seq {x1 x2} : toLabelAt Sequence.Label (SyntaxRaw ts) (.finites x1 x2) = .finite := rfl
+
+@[defeq, simp]
+theorem infinites_toLabelAt_seq {x} : toLabelAt Sequence.Label (SyntaxRaw ts) (.infinites x) = .infinite := rfl
+
+
+@[defeq, simp]
+theorem singleState_toLabelAt {s} : toLabelAt Label (SyntaxRaw ts) (singleState s) = .unique := rfl
+
+@[defeq, simp]
+theorem singleState_toLabelAt_seq {s} : toLabelAt Sequence.Label (SyntaxRaw ts) (singleState s) = .finite := rfl
+
+
+@[defeq, simp]
+theorem ellipsis_toLabelAt : toLabelAt Label _ (@ellipsis ts) = .infinites := rfl
+
+@[defeq, simp]
+theorem ellipsis_toLabelAt_seq : toLabelAt Sequence.Label _ (@ellipsis ts) = .infinite := rfl
+
+
+end Nemonuri.TransitionSystem.ExecutionFragment.SyntaxRaw
+
+end
